<?xml version="1.0"?>


<!DOCTYPE rdf:RDF [
    <!ENTITY dcterms "http://purl.org/dc/terms/" >
    <!ENTITY ro "http://purl.org/wf4ever/ro#" >
    <!ENTITY owl "http://www.w3.org/2002/07/owl#" >
    <!ENTITY dc "http://purl.org/dc/elements/1.1/" >
    <!ENTITY xsd "http://www.w3.org/2001/XMLSchema#" >
    <!ENTITY xml "http://www.w3.org/XML/1998/namespace" >
    <!ENTITY rdfs "http://www.w3.org/2000/01/rdf-schema#" >
    <!ENTITY rdf "http://www.w3.org/1999/02/22-rdf-syntax-ns#" >
    <!ENTITY result "http://www.w3.org/2001/sw/DataAccess/tests/result-set#" >
]>


<rdf:RDF xmlns="http://purl.org/minim/minim#"
     xml:base="http://purl.org/minim/minim"
     xmlns:dc="http://purl.org/dc/elements/1.1/"
     xmlns:result="http://www.w3.org/2001/sw/DataAccess/tests/result-set#"
     xmlns:rdfs="http://www.w3.org/2000/01/rdf-schema#"
     xmlns:ro="http://purl.org/wf4ever/ro#"
     xmlns:owl="http://www.w3.org/2002/07/owl#"
     xmlns:xsd="http://www.w3.org/2001/XMLSchema#"
     xmlns:rdf="http://www.w3.org/1999/02/22-rdf-syntax-ns#"
     xmlns:xml="http://www.w3.org/XML/1998/namespace"
     xmlns:dcterms="http://purl.org/dc/terms/">
    <owl:Ontology rdf:about="http://purl.org/minim/minim-results"/>
    


    <!-- 
    ///////////////////////////////////////////////////////////////////////////////////////
    //
    // Annotation properties
    //
    ///////////////////////////////////////////////////////////////////////////////////////
     -->

    


    <!-- 
    ///////////////////////////////////////////////////////////////////////////////////////
    //
    // Datatypes
    //
    ///////////////////////////////////////////////////////////////////////////////////////
     -->

    


    <!-- http://purl.org/minim/minim#string -->

    <rdfs:Datatype rdf:about="http://purl.org/minim/minim#string"/>
    


    <!-- 
    ///////////////////////////////////////////////////////////////////////////////////////
    //
    // Object Properties
    //
    ///////////////////////////////////////////////////////////////////////////////////////
     -->

    


    <!-- http://purl.org/minim/minim#fullySatisfies -->

    <owl:ObjectProperty rdf:about="http://purl.org/minim/minim#fullySatisfies">
        <rdfs:label>Fully satisfied model</rdfs:label>
        <rdfs:comment>This property is used in checklist results to relate an evaluated target resource
        with a checklist model that is fully satisfied by that resource (i.e. all MUST, SHOULD 
        and MAY requirements satisfied).</rdfs:comment>
        <rdfs:range rdf:resource="http://purl.org/minim/minim#Model"/>
        <rdfs:domain rdf:resource="&ro;Resource"/>
    </owl:ObjectProperty>
    


    <!-- http://purl.org/minim/minim#minimUri -->

    <owl:ObjectProperty rdf:about="http://purl.org/minim/minim#minimUri">
        <rdfs:label>Minim definition resource</rdfs:label>
        <rdfs:comment>This property relates a checklist result to a resource containing Minim definitions used to perform a checklist evaluation.</rdfs:comment>
        <rdfs:domain rdf:resource="http://purl.org/minim/minim#Result"/>
        <rdfs:range rdf:resource="&owl;Thing"/>
    </owl:ObjectProperty>
    


    <!-- http://purl.org/minim/minim#minimallySatisfies -->

    <owl:ObjectProperty rdf:about="http://purl.org/minim/minim#minimallySatisfies">
        <rdfs:label>Minimally satisfied model</rdfs:label>
        <rdfs:comment>This property is used in checklist results to relate an evaluated target resource
        with a checklist model that is minimally (adequately) satisfied by that resource 
        (i.e. all MUST requirements satisfied).</rdfs:comment>
        <rdfs:range rdf:resource="http://purl.org/minim/minim#Model"/>
        <rdfs:domain rdf:resource="&ro;Resource"/>
    </owl:ObjectProperty>
    


    <!-- http://purl.org/minim/minim#missingMay -->

    <owl:ObjectProperty rdf:about="http://purl.org/minim/minim#missingMay">
        <rdfs:label>Unsatisfied MAY item</rdfs:label>
        <rdfs:comment>This property is used in checklist results to relate an evaluated target resource
        with a checklist item that is not satisfied by the target resource, but which is
        defined as an item whose satisfaction is optional.</rdfs:comment>
        <rdfs:range rdf:resource="http://purl.org/minim/minim#ChecklistItemReport"/>
        <rdfs:domain rdf:resource="&ro;Resource"/>
    </owl:ObjectProperty>
    


    <!-- http://purl.org/minim/minim#missingMust -->

    <owl:ObjectProperty rdf:about="http://purl.org/minim/minim#missingMust">
        <rdfs:label>Unsatisfied MUST item</rdfs:label>
        <rdfs:comment>This property is used in checklist results to relate an evaluated target resource
        with a checklist item that is not satisfied by the target resource, but which MUST
        be satisfied for the overall checklist to be satisfied.</rdfs:comment>
        <rdfs:range rdf:resource="http://purl.org/minim/minim#ChecklistItemReport"/>
        <rdfs:domain rdf:resource="&ro;Resource"/>
    </owl:ObjectProperty>
    


    <!-- http://purl.org/minim/minim#missingShould -->

    <owl:ObjectProperty rdf:about="http://purl.org/minim/minim#missingShould">
        <rdfs:label>Unsatisfied SHOULD item</rdfs:label>
        <rdfs:comment>This property is used in checklist results to relate an evaluated target resource
        with a checklist item that is not satisfied by the target resource, but which SHOULD
        be satisfied for the overall checklist to be fully satisfied.</rdfs:comment>
        <rdfs:range rdf:resource="http://purl.org/minim/minim#ChecklistItemReport"/>
        <rdfs:domain rdf:resource="&ro;Resource"/>
    </owl:ObjectProperty>
    


    <!-- http://purl.org/minim/minim#nominallySatisfies -->

    <owl:ObjectProperty rdf:about="http://purl.org/minim/minim#nominallySatisfies">
        <rdfs:label>Nominally satisfied model</rdfs:label>
        <rdfs:comment>This property is used in checklist results to relate an evaluated target resource
        with a checklist model that is nominally (adequately) satisfied by that resource 
        (i.e. all MUST and SHOULD requirements satisfied).</rdfs:comment>
        <rdfs:range rdf:resource="http://purl.org/minim/minim#Model"/>
        <rdfs:domain rdf:resource="&ro;Resource"/>
    </owl:ObjectProperty>
    


    <!-- http://purl.org/minim/minim#satisfied -->

    <owl:ObjectProperty rdf:about="http://purl.org/minim/minim#satisfied">
        <rdfs:label>Satisfied checklist item</rdfs:label>
        <rdfs:comment>This property is used in checklist results to relate an evaluated target resource
        with a checklist item that is satisfied by that resource.</rdfs:comment>
        <rdfs:range rdf:resource="http://purl.org/minim/minim#ChecklistItemReport"/>
        <rdfs:domain rdf:resource="&ro;Resource"/>
    </owl:ObjectProperty>
    


    <!-- http://purl.org/minim/minim#testedChecklist -->

    <owl:ObjectProperty rdf:about="http://purl.org/minim/minim#testedChecklist">
        <rdfs:label>Tested checklist</rdfs:label>
        <rdfs:comment>This property relates a checklist result to a checklist against which it has been evaluated.</rdfs:comment>
        <rdfs:range rdf:resource="http://purl.org/minim/minim#Checklist"/>
        <rdfs:domain rdf:resource="http://purl.org/minim/minim#Result"/>
    </owl:ObjectProperty>
    


    <!-- http://purl.org/minim/minim#testedModel -->

    <owl:ObjectProperty rdf:about="http://purl.org/minim/minim#testedModel">
        <rdfs:label>Tested Minim model</rdfs:label>
        <rdfs:comment>This property relates a checklist result to a Minim model defning an evaluated checklist.  (The Minim model definition is contained within the resource referenced by minim:minimUri, and MAY be the same URI.  More commonly, the Minim model URI is the Minim resource URI with a fragment identifier, allowing a single Minim resource to contain multiple model (checklist) definitions.
        
        Note that the model definition is also included in the result graph returned, for ease of access.</rdfs:comment>
        <rdfs:range rdf:resource="http://purl.org/minim/minim#Model"/>
        <rdfs:domain rdf:resource="http://purl.org/minim/minim#Result"/>
    </owl:ObjectProperty>
    


    <!-- http://purl.org/minim/minim#testedRO -->

    <owl:ObjectProperty rdf:about="http://purl.org/minim/minim#testedRO">
        <rdfs:label>Tested RO</rdfs:label>
        <rdfs:comment>This property relates a checklist result to a Research Object that provides the context for the evaluation performed.</rdfs:comment>
        <rdfs:domain rdf:resource="http://purl.org/minim/minim#Result"/>
        <rdfs:range rdf:resource="&ro;ResearchObject"/>
    </owl:ObjectProperty>
    


    <!-- http://purl.org/minim/minim#testedTarget -->

    <owl:ObjectProperty rdf:about="http://purl.org/minim/minim#testedTarget">
        <rdfs:label>Tested target resource</rdfs:label>
        <rdfs:comment>This property relates a checklist result to a target resource for which checklist evaluation has been performed.</rdfs:comment>
        <rdfs:domain rdf:resource="http://purl.org/minim/minim#Result"/>
        <rdfs:range rdf:resource="&ro;Resource"/>
    </owl:ObjectProperty>
    


    <!-- http://purl.org/minim/minim#tryRequirement -->

    <owl:ObjectProperty rdf:about="http://purl.org/minim/minim#tryRequirement">
        <rdfs:label>Tested requirement</rdfs:label>
        <rdfs:comment>This property indicates a minim requirement tested by a checklist item report</rdfs:comment>
        <rdfs:domain rdf:resource="http://purl.org/minim/minim#ChecklistItemReport"/>
        <rdfs:range rdf:resource="http://purl.org/minim/minim#Requirement"/>
    </owl:ObjectProperty>
    


    <!-- http://www.w3.org/2001/sw/DataAccess/tests/result-set#binding -->

    <owl:ObjectProperty rdf:about="&result;binding"/>
    


    <!-- 
    ///////////////////////////////////////////////////////////////////////////////////////
    //
    // Data properties
    //
    ///////////////////////////////////////////////////////////////////////////////////////
     -->

    


    <!-- http://purl.org/minim/minim#testedPurpose -->

    <owl:DatatypeProperty rdf:about="http://purl.org/minim/minim#testedPurpose">
        <rdfs:label>Tested purpose</rdfs:label>
        <rdfs:comment>This property relates a checklist result to a string indicating a purpose for which evaluation has been performed.  (Note, this value is technically redundant, being accessible from the tested checklist resource, and included for convenience of reporting.)</rdfs:comment>
        <rdfs:domain rdf:resource="http://purl.org/minim/minim#Result"/>
        <rdfs:range rdf:resource="http://purl.org/minim/minim#string"/>
    </owl:DatatypeProperty>
    


    <!-- http://purl.org/minim/minim#tryMessage -->

    <owl:DatatypeProperty rdf:about="http://purl.org/minim/minim#tryMessage">
        <rdfs:label>Tested requirement message</rdfs:label>
        <rdfs:comment>This property indicates a message that described the outcome of the tested requirement</rdfs:comment>
        <rdfs:domain rdf:resource="http://purl.org/minim/minim#ChecklistItemReport"/>
        <rdfs:range rdf:resource="http://purl.org/minim/minim#string"/>
    </owl:DatatypeProperty>
    


    <!-- http://www.w3.org/2001/sw/DataAccess/tests/result-set#value -->

    <owl:DatatypeProperty rdf:about="&result;value"/>
    


    <!-- http://www.w3.org/2001/sw/DataAccess/tests/result-set#variable -->

    <owl:DatatypeProperty rdf:about="&result;variable"/>
    


    <!-- 
    ///////////////////////////////////////////////////////////////////////////////////////
    //
    // Classes
    //
    ///////////////////////////////////////////////////////////////////////////////////////
     -->

    


    <!-- http://purl.org/minim/minim#Checklist -->

    <owl:Class rdf:about="http://purl.org/minim/minim#Checklist">
        <rdfs:label>Minim checklist</rdfs:label>
        <rdfs:comment>A checklist object indicates a minim:Model to be satisfied if a target resource is to be considered suitable for some specific purpose.  As such, it links a target resource and a purpose for which it might be used with a minim:Model that must be satisfied for the resource to be considered fit for that purpose.

A Checklist may be associated directly with a target resource as the subject of a minim:hasChecklist statement, or may be associated indirectly via a URI template that is the object of an associated minim:forTargetTemplate statement.  The latter form is is more flexible as it allows a given checklist to be more easily used with multiple resources.</rdfs:comment>
    </owl:Class>
    


    <!-- http://purl.org/minim/minim#ChecklistItemReport -->

    <owl:Class rdf:about="http://purl.org/minim/minim#ChecklistItemReport">
        <rdfs:label>Checklist item report</rdfs:label>
        <owl:equivalentClass>
            <owl:Class>
                <owl:intersectionOf rdf:parseType="Collection">
                    <owl:Restriction>
                        <owl:onProperty rdf:resource="&result;binding"/>
                        <owl:allValuesFrom>
                            <owl:Class>
                                <owl:intersectionOf rdf:parseType="Collection">
                                    <owl:Restriction>
                                        <owl:onProperty rdf:resource="&result;value"/>
                                        <owl:qualifiedCardinality rdf:datatype="&xsd;nonNegativeInteger">1</owl:qualifiedCardinality>
                                        <owl:onDataRange rdf:resource="http://purl.org/minim/minim#string"/>
                                    </owl:Restriction>
                                    <owl:Restriction>
                                        <owl:onProperty rdf:resource="&result;variable"/>
                                        <owl:qualifiedCardinality rdf:datatype="&xsd;nonNegativeInteger">1</owl:qualifiedCardinality>
                                        <owl:onDataRange rdf:resource="http://purl.org/minim/minim#string"/>
                                    </owl:Restriction>
                                </owl:intersectionOf>
                            </owl:Class>
                        </owl:allValuesFrom>
                    </owl:Restriction>
                    <owl:Restriction>
                        <owl:onProperty rdf:resource="http://purl.org/minim/minim#tryRequirement"/>
                        <owl:onClass rdf:resource="http://purl.org/minim/minim#Requirement"/>
                        <owl:qualifiedCardinality rdf:datatype="&xsd;nonNegativeInteger">1</owl:qualifiedCardinality>
                    </owl:Restriction>
                    <owl:Restriction>
                        <owl:onProperty rdf:resource="http://purl.org/minim/minim#tryMessage"/>
                        <owl:qualifiedCardinality rdf:datatype="&xsd;nonNegativeInteger">1</owl:qualifiedCardinality>
                        <owl:onDataRange rdf:resource="http://purl.org/minim/minim#string"/>
                    </owl:Restriction>
                </owl:intersectionOf>
            </owl:Class>
        </owl:equivalentClass>
        <rdfs:comment>Each item within a checklist is reported separately by a report structure that
          is associated with the Research Object (@@should be target resource?) by a property
          indicating how it affects the overall evaluation: minim:satisfied, minim:missingMust,
          minim:missingShould or minim:missingMay.</rdfs:comment>
    </owl:Class>
    


    <!-- http://purl.org/minim/minim#Model -->

    <owl:Class rdf:about="http://purl.org/minim/minim#Model">
        <rdfs:label>Minim model</rdfs:label>
        <rdfs:comment>A Minim model collects a number of requirements, and associates each with a MUST, SHOULD or MAY requirement level.</rdfs:comment>
    </owl:Class>
    


    <!-- http://purl.org/minim/minim#Requirement -->

    <owl:Class rdf:about="http://purl.org/minim/minim#Requirement">
        <rdfs:label>Minim requirement</rdfs:label>
        <rdfs:comment>A Minim requirement, whose satisfaction is determined by evaluation of the indicated rule.
       
         The minim:seq value is used to order the requirement results returned, 
         to allow more consistent reporting of results.</rdfs:comment>
    </owl:Class>
    


    <!-- http://purl.org/minim/minim#Result -->

    <owl:Class rdf:about="http://purl.org/minim/minim#Result">
        <rdfs:label>Checklist result</rdfs:label>
        <owl:equivalentClass>
            <owl:Class>
                <owl:intersectionOf rdf:parseType="Collection">
                    <owl:Restriction>
                        <owl:onProperty rdf:resource="http://purl.org/minim/minim#minimUri"/>
                        <owl:cardinality rdf:datatype="&xsd;nonNegativeInteger">1</owl:cardinality>
                    </owl:Restriction>
                    <owl:Restriction>
                        <owl:onProperty rdf:resource="http://purl.org/minim/minim#testedChecklist"/>
                        <owl:onClass rdf:resource="http://purl.org/minim/minim#Checklist"/>
                        <owl:qualifiedCardinality rdf:datatype="&xsd;nonNegativeInteger">1</owl:qualifiedCardinality>
                    </owl:Restriction>
                    <owl:Restriction>
                        <owl:onProperty rdf:resource="http://purl.org/minim/minim#testedModel"/>
                        <owl:onClass rdf:resource="http://purl.org/minim/minim#Model"/>
                        <owl:qualifiedCardinality rdf:datatype="&xsd;nonNegativeInteger">1</owl:qualifiedCardinality>
                    </owl:Restriction>
                    <owl:Restriction>
                        <owl:onProperty rdf:resource="http://purl.org/minim/minim#testedRO"/>
                        <owl:onClass rdf:resource="&ro;ResearchObject"/>
                        <owl:qualifiedCardinality rdf:datatype="&xsd;nonNegativeInteger">1</owl:qualifiedCardinality>
                    </owl:Restriction>
                    <owl:Restriction>
                        <owl:onProperty rdf:resource="http://purl.org/minim/minim#testedTarget"/>
                        <owl:onClass rdf:resource="&ro;Resource"/>
                        <owl:qualifiedCardinality rdf:datatype="&xsd;nonNegativeInteger">1</owl:qualifiedCardinality>
                    </owl:Restriction>
                    <owl:Restriction>
                        <owl:onProperty rdf:resource="http://purl.org/minim/minim#testedPurpose"/>
                        <owl:qualifiedCardinality rdf:datatype="&xsd;nonNegativeInteger">1</owl:qualifiedCardinality>
                        <owl:onDataRange rdf:resource="http://purl.org/minim/minim#string"/>
                    </owl:Restriction>
                </owl:intersectionOf>
            </owl:Class>
        </owl:equivalentClass>
        <rdfs:comment>A resource the represents the result of a single checklist evaluation.</rdfs:comment>
    </owl:Class>
    


    <!-- http://purl.org/wf4ever/ro#ResearchObject -->

    <owl:Class rdf:about="&ro;ResearchObject">
        <rdfs:label>Research Object</rdfs:label>
        <rdfs:comment>Many checklist result annotations are applied to the research object that provides
          the context for the evaluation.
          
          In addition to checklist results, some useful descriptive information from the original
          data may be included with the result graph, including:  rdfs:label, 
          dctertms:identifier, dcterms:title, dcterms:description</rdfs:comment>
    </owl:Class>
    


    <!-- http://purl.org/wf4ever/ro#Resource -->

    <owl:Class rdf:about="&ro;Resource">
        <rdfs:label>RO Target resource</rdfs:label>
        <rdfs:comment>The target resource is decorated with properties that indicate the extent to which
          it satisfied a checklist.
          
          In addition, a label property from the original data may be included to help with 
          reporting of results</rdfs:comment>
    </owl:Class>
</rdf:RDF>



<!-- Generated by the OWL API (version 3.2.3.1824) http://owlapi.sourceforge.net -->

